---
ä½œè€…: è®¸å®æ°
æ—¥æœŸ: 2026-01-10
title: äºŒæ¬¡å‡½æ•°ç›¸å…³é—®é¢˜4
aliases:
tags:
ç‰ˆæƒ: Â© 2025 [è®¸å®æ°]
---
è§£æï¼š
$ç”±é¢˜å¯å¾—(m+1)x^2-(m-1)x+m-1\le x^2=2x$
$\therefore m(x^2-x+1)\le x+1$
$å³m\le \frac{x+1}{x^2-x+1}$[[ğŸ’–åˆ†å¼å‹å‡½æ•°]]
ä¸‹é¢æ±‚$\frac{x+1}{x^2-x+1}$çš„æœ€å°å€¼å³å¯
$t=x+1\in[1,3],\frac{x+1}{x^2-x+1}=\frac{t}{t^2-3t+3}=\frac{1}{t-3+\frac{3}{t}}$
$t+\frac{3}{t}-3\ge 2\sqrt3-3$
$\therefore \frac{x+1}{x^2-x+1}\le \frac{1}{2\sqrt3-3}=\frac{2\sqrt3}{3}+1$
$m\le \frac{2\sqrt3}{3}+1$


