**é¢˜ç›®5**$å·²çŸ¥å‡½æ•°f(x)=x^2-ax+a-b$
$(1)å½“a=b=2æ—¶ï¼Œæ±‚f(x)åœ¨åŒºé—´[-2,3]ä¸Šçš„æœ€å¤§å€¼ï¼›$
$(2)è‹¥\forall x\in R,f(x)\ge 0,æ±‚bçš„æœ€å¤§å€¼ï¼Œå¹¶æ±‚å½“bå–å¾—æœ€å¤§å€¼æ—¶f(b)çš„å€¼$
$(3)è‹¥\exists t\in[1,3],ä½¿å¾—f(t)=-b,æ±‚açš„å–å€¼èŒƒå›´$
è§£æï¼š
$(1)f(x)=x^2-2x,x\in[-2,3],å¯¹ç§°è½´ä¸ºx=1$
$f(x)åœ¨[-2,1]å‡ï¼Œ[1,3]å¢$
$f(-2)>f(3)$
$\therefore f(x)_max=f(-2)=8$
$(2)ç”±é¢˜å¯å¾—ï¼Œ\Delta=a^2-4(a-b)\le0$
$å³4b\le -a^2+4a=-(a-2)^2+4\le4$
$\therefore b\le1$
$æ­¤æ—¶ï¼Œa=2,f(b)=f(1)=1-2+2-1=0$
$(3)f(t)=-b\Rightarrow t^2-at+a=0åœ¨t\in[1,3]æœ‰è§£$
>[!tip]
>åˆ†ç¦»å‚æ•°[[ğŸ’–å‚å˜åˆ†ç¦»]]

$t=1æ—¶ï¼Œ1=0ï¼Œä¸æˆç«‹$
$t\neq1æ—¶ï¼Œa=\frac{t^2}{t-1}$
$æ±‚\frac{t^2}{t-1}çš„å–å€¼èŒƒå›´å³å¯$
$\frac{t^2}{t-1}=\frac{t^2-1+1}{t-1}$
$=t+1+\frac{1}{t-1}=t-1+\frac{1}{t-1}+2$
$s=t-1\in(0,2]$
$\frac{t^2}{t-1}=s+\frac{1}{s}+2\ge4$[[ğŸ’–å¯¹å‹¾å‡½æ•°]]
$\therefore a\ge4$






