è§£æžï¼š[[ðŸ’–æ¯”è¾ƒå¤§å°çš„æ–¹æ³•]]ä¸­ä¹Ÿæœ‰æž„é€ æ³•ï¼Œçœ‹çœ‹æ˜¯å¦ç›¸åŒ
>[!tip]
>ç±»æ¯”
>$\frac{f(x_1)-f(x_2)}{x_1-x_2}>0$
>æž„é€ å‡½æ•°
>$F(x)=xf(x)$
>$\frac{F(x_1)-F(x_2)}{x_1-x_2}>0$

>[!step]
>è§‚å¯Ÿ
>$f(x-1)>\frac{6}{x-1}$
>å¯åŒ–ä¸º
>$x-1>0æ—¶(x-1)f(x-1)>6$
>$x-1<0æ—¶(x-1)f(x-1)<6$
>ä¸ºäº†æ›´å¥½çš„åˆ©ç”¨å•è°ƒæ€§
>-6è¦è½¬åŒ–
>$-6=-2f(-2)$

>[!step]
>$x-1>0$
$(x-1)f(x-1)>-2f(-2)$
$å³F(x-1)>F(-2)$

>[!step]
>$x-1<0$
$(x-1)f(x-1)<-2f(-2)$
$å³F(x-1)<F(-2)$

>[!step]
>$f(x)ä¸ºå¥‡å‡½æ•°ï¼Œæ‰€ä»¥F(x)ä¸ºå¶å‡½æ•°,ä¸”åœ¨(0,+\infty)é€’å¢ž$

$\begin{cases}x-1>0\\|x-1|>|-2|\end{cases}$
æˆ–
$\begin{cases}x-1<0\\|x-1|<|-2|\end{cases}$
$-1<x<1æˆ–x>3$

>[!important]
>==ç”¨å¿ƒä½“ä¼šè¿™ä¸ªè¿‡ç¨‹==

