>[!success] å¯¹ç§°æ€§+åŸºæœ¬ä¸ç­‰å¼
>$å·²çŸ¥å‡½æ•°f(x)=\lg(\sqrt{9x^2+1}-3x)+1,æ­£å®æ•°a,bæ»¡è¶³f(2a)+f(b-4)=2$
>$æ±‚\frac{1}{a}+\frac{1}{b}çš„æœ€å°å€¼$

>[!è§£æ]
>$ä¸è¦æ€¥äºä»£å…¥ï¼Œå…ˆç ”ç©¶å‡½æ•°çš„ç‰¹å¾---æ€§è´¨æˆ–å›¾åƒ$
>$f(-x)+f(x)=2$
>>$\color{red}æ¨¡å‹f(x)=\log_a(\sqrt{ax^2+1}\pm ax)ä¸ºå¥‡å‡½æ•°$
>
>$\therefore 2a+b-4=0\Rightarrow 2a+b=4$
>$\because a,bä¸ºæ­£æ•°$
>$\frac{1}{a}+\frac{1}{b}=\frac{1}{4}(\frac{1}{a}+\frac{1}{b})(2a+b)$
>$=\frac{1}{4}(3+\frac{2a}{b}+\frac{b}{a})\ge\frac{1}{4}(3+2\sqrt2)$
>$å½“ä¸”ä»…å½“\frac{2a}{b}=\frac{b}{a}å³\begin{cases}a=4-2\sqrt2\\b=4\sqrt2-4\end{cases}æ—¶ï¼Œå–å¾—æœ€å°å€¼$

---
å‚è€ƒ[[ğŸ’–å¥‡å¶æ€§ï¼ˆå¯¹ç§°æ€§ï¼‰]]      [[å‡½æ•°æ€§è´¨]]        [[ğŸ’–é½æ¬¡åŒ–æ–¹æ³•]]



