>[!success] 指对运算
>$(1)0.064^{-\frac{1}{3}}-(-\frac{4}{5})^0+(2^3)^{-\frac{4}{3}}-2^{-4}\cdot(\sqrt3)^4$
>$(2)\log_20.25+\ln{\sqrt e}+2^{4\log_23}+2\lg5-\sqrt[4]{(-2)^4}$
>$(3)a^{\frac{1}{2}}+a^{-\frac{1}{2}}=3,求\frac{a^2+a^{-2}+3}{a+a^{-1}-2}$

>[!解析]
>$(1)0.064^{-\frac{1}{3}}-(-\frac{4}{5})^0+(2^3)^{-\frac{4}{3}}-2^{-4}\cdot(\sqrt3)^4$
>$=(0.4^3)^{-\frac{1}{3}}-1+2^{-4}-(\frac{1}{2})^{4}\cdot(3^{\frac{1}{2}})^4$
>$=(\frac{2}{5})^{-1}-1+\frac{1}{16}-\frac{9}{16}$
>$=\frac{5}{2}-1+\frac{1}{16}-\frac{9}{16}=1$
>

>[!continue]
$(2)\log_20.25+\ln{\sqrt e}+2^{4\log_23}+2\lg5-\sqrt[4]{(-2)^4}$
$=\log_2{5^{-2}}+\ln e^{\frac{1}{2}}+(2^{\log_23})^4+2\lg5-|-2|$
$=-2\log_25+\frac{1}{2}\ln e+3^4+2\lg5-2=\frac{159}{2}$

>[!continue]
>$(3)$


