>[!success] é¢˜ç›®
>$å·²çŸ¥å‡½æ•°f(x)=\begin{cases}x^2+e^x,x\ge0,\\x^2+e^{-x},x<0,\end{cases},è‹¥a=(\tan\alpha)^{\tan\alpha},b==(\sin\alpha)^{\cos\alpha},c=-(\cos)^{\sin\alpha},\alpha\in(\frac{\pi}{4},\frac{\pi}{2})$
>$åˆ™ä¸‹åˆ—ç»“è®ºæ­£ç¡®çš„æ˜¯()$
>- [ ] $A.f(a)<f(b)<f(c)$
>- [ ] $B.f(b)<f(c)<f(a)$
>- [ ] $C.f(c)<f(b)<f(a)$
>- [ ] $D.f(b)<f(a)<f(c)$

>[!ç­”æ¡ˆ]-
>$x>0æ—¶,f(x)=x^2+e^x,-x<0,f(-x)=x^2+e^xï¼Œf(-x)=f(x)$
>$åŒç†x<0æ—¶ï¼Œf(-x)=f(x),\therefore f(x)ä¸ºå¶å‡½æ•°$
>$x\ge0æ—¶ï¼Œf(x)ä¸ºå¢å‡½æ•°$
>$\alpha\in(\frac{\pi}{4},\frac{\pi}{2}),0<\cos\alpha<\sin\alpha<1<\tan\alpha$
>$åˆ™0<(\cos\alpha)^{\sin\alpha}<(\cos\alpha)^{\cos\alpha}<(\sin\alpha)^{\cos\alpha}<1,\tan\alpha>1$
>$\therefore a>b>-c>0\Rightarrow f(a>f(b)>f(-c)=f(c)$
>$ç­”æ¡ˆï¼šC$


 >[!help] æ€ç»´è¿‡ç¨‹å›¾
 >```mermaid
graph TB
A[åˆ†æ®µå‡½æ•°æ€§è´¨]
A-->B[å¥‡å¶æ€§]
A-->C[å•è°ƒæ€§]
A-->D[å¹‚å‡½æ•°å•è°ƒæ€§]
D-->E[æ¯”è¾ƒa,b,c]
F[ä¸­é—´å€¼æ¯”è¾ƒå¤§å°]-->E
G[æŒ‡æ•°å‡½æ•°å•è°ƒæ€§]-->E
C-->H["æ¯”è¾ƒf(a)å’Œf(b)"]
E-->H
H-->J
B-->I["f(-c)=f(c)"]
I-->J["æœ€ç»ˆç»“æœ"]



```
```
---
å‚è€ƒ[[ğŸ’–æ¯”è¾ƒå¤§å°çš„æ–¹æ³•]]






